src/Implementations/File/Definitions.v
@@ -1,6 +1,19 @@
-Require Import Framework LoggedDiskLayer Inode.
+Require Import Framework TransactionalDiskLayer BlockAllocator Inode.
+Import IfNotations.
 
 Open Scope pred_scope.
+
+Axiom disk_start_addr: addr.
+Axiom disk_block_count: nat.
+Axiom disk_block_count_in_bounds: disk_block_count <= block_size.
+
+Module DiskAllocatorParams <: BlockAllocatorParameters.
+  Definition bitmap_addr := disk_start_addr.
+  Definition num_of_blocks := disk_block_count.
+  Definition num_of_blocks_in_bounds := disk_block_count_in_bounds.
+End DiskAllocatorParams.
+
+Module DiskAllocator := BlockAllocator DiskAllocatorParams.
 
 Record File :=
   {
@@ -8,57 +21,99 @@ Record File :=
     blocks: list value;
   }.
 
-Definition file_rep file (inode: Inode) : @pred addr addr_dec (set value) :=
-  exists* fblocks,
-  [[ file.(owner) = inode.(Inode.Definitions.owner) ]] *
-  inode.(Inode.Definitions.blocks) |L> fblocks *
-  [[ file.(blocks) = map fst fblocks ]].
+Definition file_rep (file: File) (inode: Inode) (file_block_map: disk value) :=
+  file.(owner) = inode.(Inode.Definitions.owner) /\
+  length file.(blocks) = length inode.(block_numbers) /\
+  (forall i block_number,
+       nth_error inode.(block_numbers) i = Some block_number ->
+       nth_error file.(blocks) i = file_block_map block_number).
 
-Fixpoint file_list_inner_rep flist ilist :=
-  match flist, ilist with
-  | file::flist', inode::ilist' =>
-    file_rep file inode * file_list_inner_rep flist' ilist'
-  | _, _ => emp
-  end.
+Definition files_inner_rep file_map inode_map file_block_map :=
+   addrs_match file_map inode_map /\
+   (forall inum inode file,
+     inode_map inum  = Some inode ->
+     file_map inum = Some file ->
+     file_rep file inode file_block_map).
 
-Definition file_list_rep flist :=
-  exists* ilist,
-    inode_list_rep ilist *
-    let valid_ilist := filter (fun inode => inode.(used)) ilist in
-    [[ length flist = length valid_ilist ]] *
-    file_list_inner_rep flist valid_ilist.
+Definition files_rep (file_map: disk File) :=
+  exists* inode_map file_block_map,
+    inode_rep inode_map *
+    DiskAllocator.block_allocator_rep file_block_map *
+    [[ files_inner_rep file_map inode_map file_block_map ]].
 
-
+Definition get_block_number inum off :=
+  r <- get_inode inum;
+  if r is Some inode then
+    Ret (nth_error inode.(block_numbers) off)
+  else
+    Ret None.
+  
 Definition read inum off :=
-  inode <- get_inode inum;
-  let bn := nth off inode.(Inode.Definitions.blocks) 0 in
-  v <-| Read bn;
-  Ret v.
+  _ <-| Start;
+  r <- get_block_number inum off;
+  if r is Some block_number then
+    r <- DiskAllocator.read block_number;
+   if r is Some v then
+      _ <-| Commit;
+     Ret r
+    else
+      _ <-| Abort;
+      Ret r
+  else
+    _ <-| Abort;
+    Ret None.
 
 Definition write inum off v :=
-  inode <- get_inode inum;
-  let bn := nth off inode.(Inode.Definitions.blocks) 0 in
-  _ <-| Write [bn] [v];
-  Ret tt.
+  _ <-| Start;
+  r <- get_block_number inum off;
+  if r is Some block_number then
+    r <- DiskAllocator.write block_number v;
+    if r is Some tt then
+      _ <-| Commit;
+     Ret r
+    else
+      _ <-| Abort;
+      Ret r
+  else
+    _ <-| Abort;
+    Ret None.
 
-Definition set_owner inum owner :=
-  inode <- get_inode inum;
-  let new_inode := Build_Inode inode.(used) owner inode.(Inode.Definitions.blocks) in
-  _ <- set_inode inum new_inode;
-  Ret tt.
+Definition change_owner inum owner :=
+  _ <-| Start;
+  r <- change_owner inum owner;
+  if r is Some tt then
+     _ <-| Commit;
+     Ret r
+  else
+    _ <-| Abort;
+    Ret r.
 
 Definition create owner :=
-  minum <- get_last_unused_inum;
-  match minum with
-  | Some inum =>
-    _ <- set_inode inum (Build_Inode true owner []);
-    Ret (Some inum)
-  | None =>
-    Ret None
-  end.
+  _ <-| Start;
+  r <- alloc owner;
+  if r is Some inum then
+     _ <-| Commit;
+     Ret r
+  else
+    _ <-| Abort;
+    Ret r.
 
 Definition delete inum :=
-  inode <- get_inode inum;
-  let new_inode := Build_Inode false inode.(Inode.Definitions.owner) [] in
-  _ <- set_inode inum new_inode;
-  Ret tt.
+  _ <-| Start;
+  r <- free inum;
+  if r is Some tt then
+     _ <-| Commit;
+     Ret r
+  else
+    _ <-| Abort;
+    Ret r.
+
+Definition extend inum v :=
+  _ <-| Start;
+  r <- extend inum v;
+  if r is Some tt then
+     _ <-| Commit;
+     Ret r
+  else
+    _ <-| Abort;
+    Ret r.
