src/Refinements/TransactionalDisk/Definitions.v
@@ -1,0 +1,148 @@
+Require Import Framework TransactionCacheLayer TransactionalDiskLayer Transaction.
+Close Scope pred_scope.
+Import ListNotations.
+
+Notation "'low_op'" := TransactionCacheOperation.
+Notation "'high_op'" := TransactionalDiskOperation.
+Notation "'low'" := TransactionCacheLang.
+Notation "'high'" := TransactionalDiskLang.
+
+Fixpoint apply_list {A AEQ V} (m: @mem A AEQ V) l :=
+  match l with
+  | nil =>
+    m
+  | av :: l' =>
+    apply_list (upd m (fst av) (snd av)) l'
+  end.
+
+Fixpoint compile {T} (p2: prog high T) : prog low T.
+  destruct p2.
+  {
+    destruct p.
+    exact start.
+    exact (read a).
+    exact (write a v).
+    exact commit.
+    exact abort.
+  }
+  {
+    exact (Ret t).
+  }
+  {
+    exact (Bind (compile T p2) (fun x => compile T' (p x))).
+  }
+Defined.
+
+Fixpoint oracle_refines_to T (d1: state low) (p: prog high T) o1 o2 : Prop :=
+    match p with
+    | @Bind _ T1 T2 p1 p2 =>
+      exists o1' o1'' o2' o2'',
+      o1 = o1'++o1'' /\
+      o2 = o2' ++ o2'' /\
+     ((exists d1', exec low o1' d1 (compile p1) (Crashed d1') /\
+         oracle_refines_to T1 d1 p1 o1' o2') \/
+      (exists d1' r ret,
+         exec low o1' d1 (compile p1) (Finished d1' r) /\
+         exec low o1'' d1' (compile (p2 r)) ret /\
+         oracle_refines_to T1 d1 p1 o1' o2' /\
+         oracle_refines_to T2 d1' (p2 r) o1'' o2''
+         ))
+    |Op _ op =>
+     match op with
+     | Start =>
+       (exists d1' r,
+          exec low o1 d1 start (Finished d1' r) /\
+          o2 = [OpOracle high_op [Cont] ] /\
+          d1' = (Some [], snd d1)) \/
+       
+       (exists d1',
+          exec low o1 d1 start (Crashed d1') /\
+          ((o2 = [OpOracle high_op [CrashBefore] ] /\
+            d1' = d1) \/
+           
+           (o2 = [OpOracle high_op [CrashAfter] ] /\
+            d1' = (Some [], snd d1))))
+         
+     | Read a =>
+       (exists d1' r,
+          exec low o1 d1 (read a) (Finished d1' r) /\
+          o2 = [OpOracle high_op [Cont] ] /\
+          d1' = d1) \/
+       
+       (exists d1',
+          exec low o1 d1 (read a) (Crashed d1') /\
+          (o2 = [OpOracle high_op [CrashBefore] ] \/
+          (o2 = [OpOracle high_op [CrashAfter] ] /\
+           exists l, fst d1 = Some l /\
+           exists v, get_latest l a = Some v \/ (get_latest l a = None /\ Disk.read (snd d1) a = Some v))) /\
+          d1' = d1)
+         
+     | Write a v =>
+       (exists d1' r,
+          exec low o1 d1 (write a v) (Finished d1' r) /\          
+          o2 = [OpOracle high_op [Cont] ] /\
+          d1' = (option_map (fun l => (a, v)::l) (fst d1), snd d1)) \/
+       
+       (exists d1',
+          exec low o1 d1 (write a v) (Crashed d1') /\
+          ((o2 = [ OpOracle high_op [CrashBefore] ] /\
+            d1' = d1) \/
+           
+           (o2 = [ OpOracle high_op [CrashAfter] ] /\
+            fst d1 <> None /\
+            d1' = (option_map (fun l => (a, v)::l) (fst d1), snd d1))))
+
+     | Commit =>
+       (exists d1' r,
+          exec low o1 d1 commit (Finished d1' r) /\
+          o2 = [OpOracle high_op [Cont] ] /\
+          (exists l, fst d1 = Some l /\
+                d1' = (None, merge (apply_list empty_mem (rev l)) (snd d1)))) \/
+       
+       (exists d1',
+          exec low o1 d1 commit (Crashed d1') /\
+          ((o2 = [OpOracle high_op [CrashBefore] ] /\
+           d1' = d1) \/
+           (o2 = [OpOracle high_op [CrashAfter] ] /\
+            (exists l, fst d1 = Some l /\
+                d1' = (None,  merge (apply_list empty_mem (rev l)) (snd d1) )))))
+         
+     | Abort =>
+       (exists d1' r,
+          exec low o1 d1 abort (Finished d1' r) /\
+          o2 = [OpOracle high_op [Cont] ]) \/
+       
+       (exists d1',
+          exec low o1 d1 abort (Crashed d1') /\
+          ((o2 = [OpOracle high_op [CrashBefore] ] /\
+           d1' = d1) \/
+           (o2 = [OpOracle high_op [CrashAfter] ] /\
+          d1' = (None, snd d1))))
+     end
+
+    | Ret v =>
+      (exists d1',
+         exec low o1 d1 (Ret v) (Crashed d1') /\
+         o2 = [Language.Crash _]) \/
+      (exists d1' r,
+         exec low o1 d1 (Ret v) (Finished d1' r) /\
+         o2 = [Language.Cont _])
+    end
+.
+
+
+
+   Definition refines_to (d1: state low) (d2: state high) :=
+     fst d2 =
+     match fst d1 with
+     | Some l =>
+       apply_list empty_mem (rev l)
+     | None =>
+       empty_mem
+     end /\
+     snd d2 = snd d1.
+
+  Definition compilation_of T (p1: prog low T) (p2: prog high T) :=
+    p1 = @compile T p2.
+
+  Definition TransactionalDiskRefinement := Build_Refinement compilation_of refines_to oracle_refines_to.
